update

theories/simulang/simple_inv/adequacy.v
@@ -4,7 +4,7 @@ From iris.algebra.lib Require Import gset_bij.
 From iris.base_logic.lib Require Import gset_bij.
 From simuliris.logic Require Import satisfiable.
 From simuliris.simulation Require Import slsls closed_sim gen_log_rel.
-From simuliris.simulang Require Import proofmode tactics.
+From simuliris.simulang Require Import proofmode tactics pure_refl.
 From simuliris.simulang Require Import gen_adequacy behavior wf gen_refl.
 From simuliris.simulang.simple_inv Require Import inv refl.
 From iris.prelude Require Import options.
@@ -15,7 +15,6 @@ Class simpleGpreS Σ := {
   sbij_pre_bijG :: heapbijGpreS Σ;
 }.
 Definition simpleΣ := #[sheapΣ; heapbijΣ].
-
 Global Instance subG_sbijΣ Σ :
   subG simpleΣ Σ → simpleGpreS Σ.
 Proof. solve_inG. Qed.
@@ -52,7 +51,7 @@ Qed.
 Locate prog_ref.
 Locate ctx_ref.
 Print expr_wf.
-Print ctx_ref.
+Locate ctx_ref.
 Print log_rel.
 (** Adequacy for open terms. *)
 Theorem log_rel_adequacy Σ `{!simpleGpreS Σ} e_t e_s :
@@ -77,10 +76,11 @@ Qed.
 Definition gen_log_rel_1 `{simpleGS Σ} e_t e_s  : iProp Σ :=
   □ ∀ π (map : gmap string (val * val)) (gs : gmap string val),
     target_globals (dom gs) -∗
-    source_globals (dom gs) ==∗
+    source_globals (dom gs) -∗
     subst_map_rel val_rel (free_vars e_t ∪ free_vars e_s) map -∗
+    True -∗
     subst_map (fst <$> map) e_t ⪯{π} subst_map (snd <$> map) e_s
-      {{ λ v_t v_s, val_rel v_t v_s }}.
+      {{ λ v_t v_s, True ∗ val_rel v_t v_s }}.
 
 Print log_rel_ctx.
 Check log_rel_ctx.
@@ -88,18 +88,18 @@ Locate log_rel_ctx.
 Locate gen_log_rel_ctx.
 Locate log_rel_structural.
 
-Definition log_rel_structural_1 `{simpleGS Σ} : Prop := (∀ e_t e_s,
+Definition log_rel_structural_1 `{simpleGS Σ} (expr_head_wf : expr_head → Prop) : Prop := (∀ e_t e_s,
    let head_t := expr_split_head e_t in
    let head_s := expr_split_head e_s in
-   simulang_wf head_s.1 →
+   expr_head_wf head_s.1 →
    head_s.1 = head_t.1 →
    ([∗list] e_t';e_s' ∈ head_t.2; head_s.2, gen_log_rel_1 e_t' e_s') -∗
    gen_log_rel_1 e_t e_s).
 
-
-Theorem gen_log_rel_refl_1 `{simpleGS Σ} e :
-  log_rel_structural_1 →
-  gen_expr_wf simulang_wf e →
+Locate gen_log_rel_refl.
+Theorem gen_log_rel_refl_1 `{simpleGS Σ} e (expr_head_wf : expr_head → Prop) :
+  log_rel_structural_1 expr_head_wf →
+  gen_expr_wf expr_head_wf e →
   ⊢ gen_log_rel_1 e e.
 Proof.
   intros He Hwf.
@@ -110,17 +110,428 @@ Proof.
   all: naive_solver.
 Qed.
 
-Theorem simple_log_rel_structural_1 `{simpleGS Σ} : log_rel_structural_1.
+Local Tactic Notation "smart_sim_bind" uconstr(ctx_t) uconstr(ctx_s) uconstr(Hp) :=
+  sim_bind ctx_t ctx_s;
+  iApply (sim_wand with Hp).
+
+Locate log_rel_call.
+Lemma log_rel_call_1 `{simpleGS Σ}  e1_t e1_s e2_t e2_s :
+  (∀ π v_t v_s, ext_rel π v_t v_s ⊣⊢ True ∗ val_rel v_t v_s) →
+  gen_log_rel_1 e1_t e1_s -∗ gen_log_rel_1 e2_t e2_s -∗ gen_log_rel_1 (Call e1_t e2_t) (Call e1_s e2_s).
 Proof.
-Admitted.
-  (* intros e_t e_s ?? Hwf Hs. iIntros "IH".
+  rewrite /gen_log_rel.
+  iIntros (Hext) "#IH1 #IH2". iIntros (? xs gs) "!# #Htg #Hst #Hs Ht"; simpl.
+  smart_sim_bind (subst_map _ _) (subst_map _ _) "(IH2 [] [] [] Ht)"; eauto.
+  { iApply (subst_map_rel_weaken with "[$]"). set_solver. }
+  iIntros (v_t1 v_s1) "[Ht #Hv1]".
+  smart_sim_bind (subst_map _ _) (subst_map _ _) "(IH1 [] [] [] Ht)"; eauto.
+  { iApply (subst_map_rel_weaken with "[$]"). set_solver. }
+  iIntros (v_t2 v_s2) "[Ht #Hv2]".
+  discr_source. val_discr_source "Hv2".
+  iApply (sim_call with "[Ht]"); [done..| rewrite Hext; by iFrame| ].
+  iIntros (??) "?". iApply lift_post_val. rewrite Hext. by iFrame.
+Qed.
+
+Lemma log_rel_val `{simpleGS Σ} v_t v_s :
+  val_rel v_t v_s -∗ gen_log_rel_1 (Val v_t) (Val v_s).
+Proof.
+  rewrite /gen_log_rel.
+  iIntros "#Hv" (? xs gs) "!# Hgs Hgt Hs Ht"; simpl. sim_val; by iFrame.
+Qed.
+
+Locate log_rel_let.
+Lemma log_rel_var `{simpleGS Σ} x : ⊢ gen_log_rel_1 (Var x) (Var x).
+Proof.
+  rewrite /gen_log_rel.
+  iIntros (? xs gs) "!# Hgs Hgt Hs Ht"; simpl.
+  iDestruct (subst_map_rel_lookup _ x with "Hs") as (v_t v_s Hv) "Hrel"; first set_solver.
+  rewrite !lookup_fmap Hv /=. sim_val. by iFrame.
+Qed.
+
+Locate pure_log_rel_structural.
+Check sheap_inv_contains_globalbij.
+Locate sim_global_var.
+Lemma log_rel_global_var `{simpleGS Σ} x :
+  sheap_inv_contains_globalbij heapbij.loc_rel →
+  ⊢ gen_log_rel_1 (GlobalVar x) (GlobalVar x).
+Proof.
+  rewrite /log_rel /gen_log_rel.
+  iIntros (Hrel ? xs gs) "!# Hgs Hgt Hs Ht"; simpl.
+  iApply (sim_global_var heapbij.loc_rel); first done. iIntros (??) "Hrel".
+  iApply lift_post_val. iFrame.
+Qed.
+
+Lemma log_rel_let `{simpleGS Σ} x e1_t e1_s e2_t e2_s :
+  gen_log_rel_1 e1_t e1_s -∗ gen_log_rel_1 e2_t e2_s -∗ gen_log_rel_1 (Let x e1_t e2_t) (Let x e1_s e2_s).
+Proof.
+  unfold gen_log_rel_1.
+  iIntros "#IH1 #IH2" (? xs gs) "!# #Hgs #Hgt #Hs Ht"; simpl.
+  smart_sim_bind (subst_map _ _) (subst_map _ _) "(IH1 [] [] [Hs] Ht)"; eauto.
+  { iApply (subst_map_rel_weaken with "[$]"). set_solver. }
+  iIntros (v_t v_s) "[Ht #Hv]". sim_pures. rewrite !subst'_subst_map.
+  rewrite -(binder_insert_fmap fst (v_t, v_s)).
+  rewrite -(binder_insert_fmap snd (v_t, v_s)).
+  iApply ("IH2" with "[] [] [] Ht"); eauto.
+  iApply (subst_map_rel_insert with "[]  [Hv]"); last done.
+  iApply (subst_map_rel_weaken with "[$]").
+  destruct x as [|x]; first set_solver.
+  apply elem_of_subseteq=>x'.
+  destruct (decide (x = x')) as [<-|Hne]; set_solver.
+Qed.
+
+Lemma log_rel_unop `{simpleGS Σ} e_t e_s o :
+  gen_log_rel_1 e_t e_s -∗ gen_log_rel_1 (UnOp o e_t) (UnOp o e_s).
+Proof.
+  unfold gen_log_rel_1.
+  iIntros "#IH" (? xs gs) "!# #Hgs #Hgt #Hs Ht"; simpl.
+  smart_sim_bind (subst_map _ e_t) (subst_map _ e_s) "(IH [] [] [Hs] Ht)"; eauto.
+  (* { iApply (subst_map_rel_weaken with "[$]"). set_solver. } *)
+  iIntros (v_t v_s) "[Ht Hv]".
+  destruct o; sim_pures; discr_source; val_discr_source "Hv"; sim_pures; sim_val; by iFrame.
+Qed.
+
+Lemma log_rel_binop `{simpleGS Σ} e1_t e1_s e2_t e2_s o :
+  loc_rel_func_law heapbij.loc_rel →
+  loc_rel_inj_law heapbij.loc_rel →
+  loc_rel_offset_law heapbij.loc_rel →
+  gen_log_rel_1 e1_t e1_s -∗ gen_log_rel_1 e2_t e2_s -∗ gen_log_rel_1 (BinOp o e1_t e2_t) (BinOp o e1_s e2_s).
+Proof.
+  unfold gen_log_rel_1.
+  iIntros (Hfunc Hinj Hshift). iIntros "#IH1 #IH2" (? xs gs) "!# #Hgs #Hgt #Hs Ht"; simpl.
+  smart_sim_bind (subst_map _ e2_t) (subst_map _ e2_s) "(IH2 [] [] [] Ht)"; eauto.
+  { iApply (subst_map_rel_weaken with "[$]"). set_solver. }
+  iIntros (v_t2 v_s2) "[Ht Hv2]".
+  smart_sim_bind (subst_map _ e1_t) (subst_map _ e1_s) "(IH1 [] [] [] Ht)"; eauto.
+  { iApply (subst_map_rel_weaken with "[$]"). set_solver. }
+  iIntros (v_t1 v_s1) "[Ht Hv1]".
+  destruct o; sim_pures; discr_source; try val_discr_source "Hv1"; try val_discr_source "Hv2"; sim_pures; try (sim_val; by iFrame); [| | |].
+  - (* Quot *)
+    source_binop.
+    { rewrite /bin_op_eval /=. rewrite decide_False //. }
+    target_binop.
+    { rewrite /bin_op_eval /=. rewrite decide_False //. }
+    sim_val; by iFrame.
+  - (* Rem *)
+    source_binop.
+    { rewrite /bin_op_eval /=. rewrite decide_False //. }
+    target_binop.
+    { rewrite /bin_op_eval /=. rewrite decide_False //. }
+    sim_val; by iFrame.
+  - (* Eq *)
+    iAssert (⌜vals_compare_safe v_t1 v_t2⌝)%I as "%".
+    { iPoseProof (gen_val_rel_val_is_unboxed with "Hv1") as "%Hv1".
+      iPoseProof (gen_val_rel_val_is_unboxed with "Hv2") as "%Hv2".
+      iPureIntro. by rewrite /vals_compare_safe Hv1 Hv2.
+    }
+    sim_pures; sim_val. iFrame. case_bool_decide; subst.
+    * iDestruct (gen_val_rel_func with "Hv1 Hv2") as %->; [done|]. by case_bool_decide.
+    * case_bool_decide; [|done]; subst. by iDestruct (gen_val_rel_inj with "Hv1 Hv2") as %?.
+  - (* Offset *)
+    sim_val. iModIntro; simpl. iFrame. by iApply Hshift.
+Qed.
+
+Lemma log_rel_if `{simpleGS Σ} e1_t e1_s e2_t e2_s e3_t e3_s :
+  gen_log_rel_1 e1_t e1_s -∗
+  gen_log_rel_1 e2_t e2_s -∗
+  gen_log_rel_1 e3_t e3_s -∗
+  gen_log_rel_1 (If e1_t e2_t e3_t) (If e1_s e2_s e3_s).
+Proof.
+  unfold gen_log_rel_1.
+  iIntros "#IH1 #IH2 #IH3" (? xs gs) "!# #Hgs #Hgt #Hs Ht"; simpl.
+  smart_sim_bind (subst_map _ e1_t) (subst_map _ e1_s) "(IH1 [] [] [] Ht)"; eauto.
+  { iApply (subst_map_rel_weaken with "[$]"). set_solver. }
+  iIntros (v_t v_s) "[Ht Hv]".
+  discr_source. val_discr_source "Hv". rename select bool into b.
+  destruct b; sim_pures.
+  + iApply ("IH2" with "[] [] [] Ht"); eauto. iApply (subst_map_rel_weaken with "[$]"). set_solver.
+  + iApply ("IH3" with "[] [] [] Ht"); eauto. iApply (subst_map_rel_weaken with "[$]"). set_solver.
+Qed.
+
+Lemma log_rel_while `{simpleGS Σ} e1_t e1_s e2_t e2_s :
+  gen_log_rel_1 e1_t e1_s -∗
+  gen_log_rel_1 e2_t e2_s -∗
+  gen_log_rel_1 (While e1_t e2_t) (While e1_s e2_s).
+Proof.
+  unfold gen_log_rel_1.
+  iIntros "#IH1 #IH2" (? xs gs) "!# #Hgs #Hgt #Hs Ht"; simpl.
+  iApply (sim_while_while True with "[$]"); eauto.
+  iModIntro; iIntros "Ht".
+  smart_sim_bind (subst_map _ e1_t) (subst_map _ e1_s) "(IH1 [] [] [] Ht)"; eauto.
+  { iApply (subst_map_rel_weaken with "[$]"). set_solver. }
+  iIntros (v_t v_s) "[Ht Hv]".
+  discr_source. val_discr_source "Hv".
+  rename select bool into b.
+  destruct b; sim_pures.
+  + smart_sim_bind (subst_map _ e2_t) (subst_map _ e2_s) "(IH2 [] [] [] Ht)"; eauto.
+    { iApply (subst_map_rel_weaken with "[$]"). set_solver. }
+    iIntros (? ?) "[Ht _]"; sim_pures. iApply sim_expr_base. iRight. by eauto.
+  + iApply sim_expr_base. iLeft. iExists #(), #(); eauto.
+Qed.
+
+
+Lemma log_rel_pair `{simpleGS Σ} e1_t e1_s e2_t e2_s :
+  gen_log_rel_1 e1_t e1_s -∗
+  gen_log_rel_1 e2_t e2_s -∗
+  gen_log_rel_1 (Pair e1_t e2_t) (Pair e1_s e2_s).
+Proof.
+  rewrite /gen_log_rel.
+  iIntros "#IH1 #IH2" (? xs gs) "!# #Hgs #Hgt #Hs Ht"; simpl.
+  smart_sim_bind (subst_map _ e2_t) (subst_map _ e2_s) "(IH2 [] [] [] Ht)"; eauto.
+  { iApply (subst_map_rel_weaken with "[$]"). set_solver. }
+  iIntros (v_t2 v_s2) "[Ht Hv2]".
+  smart_sim_bind (subst_map _ e1_t) (subst_map _ e1_s) "(IH1 [] [] [] Ht)"; eauto.
+  { iApply (subst_map_rel_weaken with "[$]"). set_solver. }
+  iIntros (v_t1 v_s1) "[Ht Hv1]".
+  sim_pures; sim_val. by iFrame.
+Qed.
+
+Lemma log_rel_fst `{simpleGS Σ} e_t e_s :
+  gen_log_rel_1 e_t e_s -∗ gen_log_rel_1 (Fst e_t) (Fst e_s).
+Proof.
+  rewrite /gen_log_rel.
+  iIntros "#IH" (? xs gs) "!# #Hgs #Hgt Hs Ht"; simpl.
+  smart_sim_bind (subst_map _ e_t) (subst_map _ e_s) "(IH [] [] [Hs] Ht)"; eauto.
+  (* { iApply (subst_map_rel_weaken with "[$]"). set_solver. } *)
+  iIntros (v_t v_s) "[Ht Hv]".
+  discr_source.
+  iPoseProof (gen_val_rel_pair_source with "Hv") as (??) "(-> & ? & ?)"; sim_pures; sim_val; by iFrame.
+Qed.
+
+Lemma log_rel_snd `{simpleGS Σ} e_t e_s :
+  gen_log_rel_1 e_t e_s -∗ gen_log_rel_1 (Snd e_t) (Snd e_s).
+Proof.
+  rewrite /gen_log_rel.
+  iIntros "#IH" (? xs gs) "!# #Hgs #Hgt Hs Ht"; simpl.
+  smart_sim_bind (subst_map _ e_t) (subst_map _ e_s) "(IH [] [] [Hs] Ht)"; eauto.
+  (* { iApply (subst_map_rel_weaken with "[$]"). set_solver. } *)
+  iIntros (v_t v_s) "[Ht Hv]".
+  discr_source.
+  iPoseProof (gen_val_rel_pair_source with "Hv") as (??) "(-> & ? & ?)"; sim_pures; sim_val; by iFrame.
+Qed.
+
+Lemma log_rel_injl `{simpleGS Σ} e_t e_s :
+  gen_log_rel_1 e_t e_s -∗ gen_log_rel_1 (InjL e_t) (InjL e_s).
+Proof.
+  unfold gen_log_rel_1.
+  iIntros "#IH" (? xs gs) "!# #Hgs #Hgt #Hs Ht"; simpl.
+  smart_sim_bind (subst_map _ e_t) (subst_map _ e_s) "(IH [] [] [] Ht)"; eauto.
+  iIntros (v_t v_s) "[Ht Hv]"; sim_pures; sim_val; by iFrame.
+Qed.
+
+Lemma log_rel_injr `{simpleGS Σ} e_t e_s :
+  gen_log_rel_1 e_t e_s -∗ gen_log_rel_1 (InjR e_t) (InjR e_s).
+Proof.
+  unfold gen_log_rel_1.
+  iIntros "#IH" (? xs gs) "!# #Hgs #Hgt #Hs Ht"; simpl.
+  smart_sim_bind (subst_map _ e_t) (subst_map _ e_s) "(IH [] [] [] Ht)"; eauto.
+  iIntros (v_t v_s) "[Ht Hv]"; sim_pures; sim_val; by iFrame.
+Qed.
+
+Lemma log_rel_match `{simpleGS Σ} e_t e_s e1_t e1_s e2_t e2_s x1 x2 :
+  gen_log_rel_1 e_t e_s -∗
+  gen_log_rel_1 e1_t e1_s -∗
+  gen_log_rel_1 e2_t e2_s -∗
+  gen_log_rel_1 (Match e_t x1 e1_t x2 e2_t) (Match e_s x1 e1_s x2 e2_s).
+Proof.
+  unfold gen_log_rel_1.
+  iIntros "#IH #IH1 #IH2" (? xs gs) "!# #Hgs #Hgt #Hs Ht"; simpl.
+  smart_sim_bind (subst_map _ e_t) (subst_map _ e_s)  "(IH [] [] [] Ht)"; eauto.
+  { iApply (subst_map_rel_weaken with "[$]"). set_solver. }
+  iIntros (v_t v_s) "[Ht #Hv]".
+  discr_source.
+  + iPoseProof (gen_val_rel_injl_source with "Hv") as (v_t') "(-> & ?)". sim_pures.
+    rewrite !subst'_subst_map.
+    match goal with |- context[gen_val_rel loc_rel (InjLV ?vt) (InjLV ?vs)] =>
+      rename vt into v_t'; rename vs into v_s'
+    end.
+    rewrite -(binder_insert_fmap fst (v_t', v_s')).
+    rewrite -(binder_insert_fmap snd (v_t', v_s')).
+    iApply ("IH1" with "[] [] [] Ht"); eauto.
+    iApply (subst_map_rel_insert with "[] []"); last done.
+    iApply (subst_map_rel_weaken with "[$]").
+    destruct x1 as [|x1]; first set_solver.
+    apply elem_of_subseteq=>x'.
+    destruct (decide (x1 = x')) as [<-|Hne]; set_solver.
+  + iPoseProof (gen_val_rel_injr_source with "Hv") as (v_t') "(-> & ?)". sim_pures.
+    rewrite !subst'_subst_map.
+    match goal with |- context[gen_val_rel loc_rel (InjRV ?vt) (InjRV ?vs)] =>
+      rename vt into v_t'; rename vs into v_s'
+    end.
+    rewrite -(binder_insert_fmap fst (v_t', v_s')).
+    rewrite -(binder_insert_fmap snd (v_t', v_s')).
+    iApply ("IH2" with "[] [] [] Ht"); eauto.
+    iApply (subst_map_rel_insert with "[] []"); last done.
+    iApply (subst_map_rel_weaken with "[$]").
+    destruct x2 as [|x2]; first set_solver.
+    apply elem_of_subseteq=>x'.
+    destruct (decide (x2 = x')) as [<-|Hne]; set_solver.
+Qed.
+
+Definition thread_own `{simpleGS Σ} : thread_id → iProp Σ := λ _ : thread_id, True%I.
+Lemma log_rel_fork `{simpleGS Σ} e_t e_s :
+  (∀ e_s e_t π Ψ,
+   thread_own π -∗
+   (thread_own π -∗ #() ⪯{π} #() [{ Ψ }]) -∗
+   (∀ π', thread_own π' -∗ e_t ⪯{π'} e_s {{ λ v_t v_s, thread_own π' ∗ val_rel v_t v_s }}) -∗
+   Fork e_t ⪯{π} Fork e_s [{ Ψ }]) →
+  gen_log_rel_1 e_t e_s -∗ gen_log_rel_1 (Fork e_t) (Fork e_s).
+Proof.
+  unfold gen_log_rel_1.
+  iIntros (Hfork). iIntros "#IH" (? xs gs) "!# #Hgs #Hgt #Hs Ht"; simpl.
+  iApply (Hfork with "Ht"); first by iIntros "?"; sim_pures; sim_val; iFrame.
+  iIntros (?) "Ht". iApply (sim_wand with "(IH [] [] [] Ht)"); eauto.
+Qed.
+
+Lemma log_rel_allocN `{simpleGS Σ} e1_t e1_s e2_t e2_s :
+  (∀ (n : Z) v_t v_s π Ψ, (0 < n)%Z →
+   thread_own π -∗ val_rel v_t v_s -∗
+   (∀ l_t l_s, thread_own π -∗ loc_rel l_t l_s -∗ #l_t ⪯{π} #l_s [{ Ψ }]) -∗
+   AllocN #n v_t ⪯{π} AllocN #n v_s [{ Ψ }]) →
+  gen_log_rel_1 e1_t e1_s -∗ gen_log_rel_1 e2_t e2_s -∗ gen_log_rel_1 (AllocN e1_t e2_t) (AllocN e1_s e2_s).
+Proof.
+  rewrite /gen_log_rel.
+  iIntros (Halloc). iIntros "#IH1 #IH2" (? xs gs) "!# #Hs #Hgs #Hgt Ht"; simpl.
+  smart_sim_bind (subst_map _ e2_t) (subst_map _ e2_s) "(IH2 [] [] [] Ht)"; eauto.
+  { iApply (subst_map_rel_weaken with "[$]"). set_solver. }
+  iIntros (v_t v_s) "[Ht Hv]".
+  smart_sim_bind (subst_map _ e1_t) (subst_map _ e1_s) "(IH1 [] [] [] Ht)"; eauto.
+  { iApply (subst_map_rel_weaken with "[$]"). set_solver. }
+  iIntros (v_t' v_s') "[Ht Hv']".
+  discr_source. val_discr_source "Hv'".
+  iApply (Halloc with "Ht Hv"); [done|].
+  iIntros (l_t l_s) "Ht Hl". sim_val. by iFrame.
+Qed.
+
+Lemma log_rel_freeN `{simpleGS Σ} e1_t e1_s e2_t e2_s :
+  (∀ (n : Z) l_t l_s π Ψ, (0 < n)%Z →
+   thread_own π -∗ loc_rel l_t l_s -∗
+   (thread_own π -∗ #() ⪯{π} #() [{ Ψ }]) -∗
+   FreeN #n #l_t ⪯{π} FreeN #n #l_s [{ Ψ }]) →
+  gen_log_rel_1 e1_t e1_s -∗ gen_log_rel_1 e2_t e2_s -∗ gen_log_rel_1 (FreeN e1_t e2_t) (FreeN e1_s e2_s).
+Proof.
+  rewrite /gen_log_rel.
+  iIntros (Hfree). iIntros "#IH1 #IH2" (? xs gs) "!# #Hgs #Hgt #Hs Ht"; simpl.
+  smart_sim_bind (subst_map _ _) (subst_map _ _) "(IH2 [] [] [] Ht)"; eauto.
+  { iApply (subst_map_rel_weaken with "[$]"). set_solver. }
+  iIntros (v_t v_s) "[Ht Hv]".
+  smart_sim_bind (subst_map _ _) (subst_map _ _) "(IH1 [] [] [] Ht)"; eauto.
+  { iApply (subst_map_rel_weaken with "[$]"). set_solver. }
+  iIntros (v_t' v_s') "[Ht Hv']".
+  discr_source. iPoseProof (gen_val_rel_loc_source with "Hv") as (l_t) "(-> & Hrel)".
+  iPoseProof (gen_val_rel_litint_source with "Hv'") as "->".
+  iApply (Hfree with "Ht Hrel"); [done|].
+  iIntros "Ht". sim_val. by iFrame.
+Qed.
+
+Lemma log_rel_load `{simpleGS Σ} o e_t e_s :
+  (∀ l_t l_s π Ψ,
+   thread_own π -∗ loc_rel l_t l_s -∗
+   (∀ v_t v_s, thread_own π -∗ val_rel v_t v_s -∗ v_t ⪯{π} v_s [{ Ψ }]) -∗
+   Load o #l_t ⪯{π} Load o #l_s [{ Ψ }]) →
+  gen_log_rel_1 e_t e_s -∗ gen_log_rel_1 (Load o e_t) (Load o e_s).
+Proof.
+  unfold gen_log_rel_1.
+  iIntros (Hload). iIntros "#IH" (? xs gs) "!# #Hgs #Hgt #Hs Ht"; simpl.
+  smart_sim_bind (subst_map _ _) (subst_map _ _) "(IH [] [] [] Ht)"; eauto.
+  iIntros (v_t v_s) "[Ht Hv]". discr_source.
+  iPoseProof (gen_val_rel_loc_source with "Hv") as (l_t) "(-> & Hrel)".
+  iApply (Hload with "Ht Hrel").
+  iIntros (v_t v_s) "Ht Hrel". sim_val; by iFrame.
+Qed.
+
+Lemma log_rel_store `{simpleGS Σ} o e1_t e1_s e2_t e2_s :
+  (∀ l_t l_s v_s v_t π Ψ,
+   thread_own π -∗ loc_rel l_t l_s -∗ val_rel v_t v_s -∗
+   (thread_own π -∗ #() ⪯{π} #() [{ Ψ }]) -∗
+   Store o #l_t v_t ⪯{π} Store o #l_s v_s [{ Ψ }]) →
+  gen_log_rel_1 e1_t e1_s -∗ gen_log_rel_1 e2_t e2_s -∗ gen_log_rel_1 (Store o e1_t e2_t) (Store o e1_s e2_s).
+Proof.
+  unfold gen_log_rel_1.
+  iIntros (Hstore). iIntros "#IH1 #IH2" (? xs gs) "!# #Hgs #Hgt #Hs Ht"; simpl.
+  smart_sim_bind (subst_map _ _) (subst_map _ _) "(IH2 [] [] [] Ht)"; eauto.
+  { iApply (subst_map_rel_weaken with "[$]"). set_solver. }
+  iIntros (v_t v_s) "[Ht Hv]". (* FIXME: fix printing *)
+  smart_sim_bind (subst_map _ _) (subst_map _ _) "(IH1 [] [] [] Ht)"; eauto.
+  { iApply (subst_map_rel_weaken with "[$]"). set_solver. }
+  iIntros (v_t' v_s') "[Ht Hv']".
+  discr_source. iPoseProof (gen_val_rel_loc_source with "Hv'") as (l_t) "(-> & Hrel)".
+  iApply (Hstore with "Ht Hrel Hv").
+  iIntros "Ht". sim_val; by iFrame.
+Qed.
+
+Check gen_log_rel_1.
+Lemma gen_log_rel_singleton `{simpleGS Σ} e_t e_s v_t v_s arg π (gs : gmap string val) :
+  free_vars e_t ∪ free_vars e_s ⊆ {[ arg ]} →
+  target_globals (dom gs) -∗
+  source_globals (dom gs) -∗
+  gen_log_rel_1 e_t e_s -∗
+  val_rel v_t v_s -∗
+  thread_own π -∗
+  subst_map {[arg := v_t]} e_t ⪯{π} subst_map {[arg := v_s]} e_s
+    {{ λ v_t v_s, thread_own π ∗ val_rel v_t v_s }}.
+Proof.
+  iIntros (?) "Hgt Hgs Hlog Hval Hπ".
+  unfold gen_log_rel_1.
+  iDestruct ("Hlog" $! _ {[arg := (v_t, v_s)]} gs with "[Hgt] [Hgs] [Hval] Hπ") as "Hsim"; eauto.
+  { by iApply subst_map_rel_singleton. }
+  rewrite !map_fmap_singleton. done.
+Qed.
+
+Lemma gen_log_rel_func `{simpleGS Σ} x e_t e_s (gs : gmap string val) :
+  (∀ v_t v_s π, ext_rel π v_t v_s ⊣⊢ thread_own π ∗ val_rel v_t v_s) →
+  free_vars e_t ∪ free_vars e_s ⊆ {[x]} →
+  target_globals (dom gs) -∗
+  source_globals (dom gs) -∗
+  gen_log_rel_1 e_t e_s -∗
+  func_rel (Λ:=simp_lang) (x, e_t) (x, e_s).
+Proof.
+  iIntros (Hext_val Hvars) "Hgt Hgs Hlog %v_t %v_s %π".
+  rewrite Hext_val. iIntros "[Hthread Hval]".
+  iApply (sim_wand with "[-]").
+  - rewrite /= /apply_func /= -!subst_map_singleton.
+    iApply (gen_log_rel_singleton with "Hgt Hgs Hlog Hval Hthread"); done.
+  - setoid_rewrite <- Hext_val. eauto.
+Qed.
+
+Theorem pure_log_rel_structural `{simpleGS Σ} :
+  loc_rel_func_law loc_rel →
+  loc_rel_inj_law loc_rel →
+  loc_rel_offset_law loc_rel →
+  sheap_inv_contains_globalbij loc_rel →
+  log_rel_structural_1 pure_expr_head_wf.
+Proof.
+  intros ???? e_t e_s head_t head_s Hwf Hs. iIntros "IH".
+  destruct e_t; simpl in Hs; destruct e_s => //=; simpl in Hs; simplify_eq.
+  all: try iDestruct "IH" as "[IH IH1]".
+  all: try iDestruct "IH1" as "[IH1 IH2]".
+  all: try iDestruct "IH2" as "[IH2 IH3]".
+  - (* Val *) iApply log_rel_val. by iApply val_wf_sound.
+  - (* Var *) by iApply log_rel_var.
+  - (* GlobalVar *) by iApply log_rel_global_var.
+  - (* Let *) by iApply (log_rel_let with "IH IH1").
+  - (* UnOp *) by iApply (log_rel_unop with "IH").
+  - (* BinOp *) by iApply (log_rel_binop with "IH IH1").
+  - (* If *) by iApply (log_rel_if with "IH IH1 IH2").
+  - (* While *) by iApply (log_rel_while with "IH IH1").
+  - (* Pairs *) by iApply (log_rel_pair with "IH IH1").
+  - (* Fst *) by iApply (log_rel_fst with "IH").
+  - (* Snd *) by iApply (log_rel_snd with "IH").
+  - (* InjL *) by iApply (log_rel_injl with "IH").
+  - (* InjR *) by iApply (log_rel_injr with "IH").
+  - (* Match *) by iApply (log_rel_match with "IH IH1 IH2").
+Qed.
+
+Locate simple_log_rel_structural.
+Theorem simple_log_rel_structural_1 `{simpleGS Σ} : log_rel_structural_1 simulang_wf.
+Proof.
+  intros e_t e_s ?? Hwf Hs. iIntros "IH".
   destruct e_s, e_t => //; simpl in Hs; simplify_eq.
   all: try by iApply pure_log_rel_structural; unfold loc_rel_func_law, loc_rel_inj_law, loc_rel_offset_law; eauto using heapbij_loc_func, heapbij_loc_inj, heapbij_loc_shift, sim_bij_contains_globalbij.
   all: try iDestruct "IH" as "[IH IH1]".
   all: try iDestruct "IH1" as "[IH1 IH2]".
   all: try iDestruct "IH2" as "[IH2 IH3]".
   - (* Call *)
-    iApply (log_rel_call with "IH IH1").
+    iApply (log_rel_call_1 with "IH IH1").
     iIntros (???). rewrite /= left_id. auto.
   - (* Fork *)
     iApply (log_rel_fork with "IH").
@@ -148,7 +559,7 @@ Admitted.
   - (* Store *)
     iApply (log_rel_store with "IH IH1").
     iIntros (???????) "Hl Hv Hcont". iApply (sim_bij_store with "Hl Hv"). by iApply "Hcont".
-Qed. *)
+Qed.
 
 Corollary log_rel_ctx `{simpleGS Σ} C e_t e_s :
   ctx_wf C →
@@ -167,8 +578,28 @@ Proof.
   all: naive_solver.
 Qed.
 
-Theorem log_rel_adequacy_1 Σ `{!simpleGpreS Σ} e_t e_s :
-  (∀ `(simpleGS Σ), ⊢ gen_log_rel_1 e_t e_s) →
+Locate func_rel.
+Lemma log_rel_func `{simpleGS Σ} (x : string) e_t e_s (gs : gmap string val) :
+  free_vars e_t ∪ free_vars e_s ⊆ {[x]} →
+  target_globals (dom gs) -∗
+  source_globals (dom gs) -∗
+  gen_log_rel_1 e_t e_s -∗
+  func_rel (Λ:=simp_lang) (x, e_t) (x, e_s).
+Proof.
+  apply gen_log_rel_func.
+  iIntros (v_t v_s π). rewrite /= left_id. eauto.
+Qed.
+
+Locate gen_log_rel_func.
+Print ctx_ref.
+Print prog_ref.
+Locate log_rel_func.
+Locate ctx_ref.
+Theorem log_rel_adequacy_1 Σ `{!simpleGpreS Σ} e_t e_s (gss : gmap string val) :
+  (∀ `(simpleGS Σ), ⊢ 
+    target_globals (dom gss) -∗
+    source_globals (dom gss) -∗
+    gen_log_rel_1 e_t e_s) →
   ctx_ref e_t e_s.
 Proof.
   intros Hrel C fname x p Hpwf HCwf Hvars.
@@ -177,7 +608,7 @@ Proof.
   iSplit.
   { iApply big_sepM_intro. iIntros "!>" (???). iApply val_wf_sound. by apply: Hgs. }
   iApply prog_rel_refl_insert.
-  - iModIntro. iApply log_rel_func; first done.
+  - iModIntro. unfold func_rel.  apply gen_log_rel_func.
     iApply log_rel_ctx; first done. iApply Hrel.
   - iIntros "!# %f %fn %Hfn". destruct fn as [arg body].
     destruct (Hpwf _ _ Hfn) as [Hfn_wf Hfn_vars].
